src/cbor/pulse/CBOR.Pulse.API.Det.C.Copy.fsti
@@ -3,12 +3,12 @@ include CBOR.Pulse.API.Det.C
 open Pulse.Lib.Pervasives
 
 [@@CAbstractStruct]
-val freeable_cbor_det_t: Type0
+val cbor_det_freeable_t: Type0
 
-val freeable: freeable_cbor_det_t -> slprop
+val freeable: cbor_det_freeable_t -> slprop
 
-val get_cbor_from_freeable: freeable_cbor_det_t -> cbor_det_t
+val cbor_get_from_freeable: cbor_det_freeable_t -> cbor_det_t
 
-val cbor_copy () : cbor_copy_t cbor_det_match freeable get_cbor_from_freeable
+val cbor_copy () : cbor_copy_t cbor_det_match freeable cbor_get_from_freeable
 
 val cbor_free () : cbor_free_t freeable
